src/syntax/FStarC.Syntax.CheckLN.fst
@@ -85,8 +85,6 @@ and is_ln'_bv (n:int) (bv:bv) : ML bool =
 
 and is_ln'_comp (n:int) (c:comp) : ML bool =
   match c.n with
-  | Total t -> is_ln' n t
-  | GTotal t -> is_ln' n t
   | Comp ct -> is_ln'_comp_typ n ct
 
 and is_ln'_comp_typ (n:nat) (ct:comp_typ) : ML bool =
