src/syntax/FStarC.Syntax.Hash.fst
@@ -137,14 +137,6 @@ and hash_term' (t:term)
 and hash_comp' (c:comp)
   : ML (mm H.hash_code)
   = match c.n with
-    | Total t ->
-      mix_list_lit
-        [of_int 811;
-         hash_term t]
-    | GTotal t ->
-      mix_list_lit
-        [of_int 821;
-         hash_term t]
     | Comp ct ->
       mix_list_lit
         [of_int 823;
@@ -470,15 +462,11 @@ and equal_comp c1 c2
   =
   if physical_equality c1 c2 then true else
   match c1.n, c2.n with
-  | Total t1, Total t2
-  | GTotal t1, GTotal t2 ->
-    equal_term t1 t2
   | Comp ct1, Comp ct2 ->
     Ident.lid_equals ct1.effect_name ct2.effect_name &&
     equal_list equal_universe ct1.comp_univs ct2.comp_univs &&
     equal_term ct1.result_typ ct2.result_typ &&
     equal_list equal_flag ct1.flags ct2.flags
-  | _ -> false
 
 and equal_binder b1 b2
   : ML bool
