src/typechecker/FStarC.TypeChecker.TermEqAndSimplify.fst
@@ -276,9 +276,6 @@ and eq_args env (a1:args) (a2:args) : ML eq_result =
 
 and eq_comp env (c1 c2:comp) : ML eq_result =
   match c1.n, c2.n with
-  | Total t1, Total t2
-  | GTotal t1, GTotal t2 ->
-    eq_tm env t1 t2
   | Comp ct1, Comp ct2 ->
     eq_and (equal_if (eq_univs_list ct1.comp_univs ct2.comp_univs))
            (fun _ ->
